ex_proof_rules.thy
@@ -9,6 +9,15 @@ text "We first define partial correctness of a program with pre- and post-condit
 definition correct :: "(state \<Rightarrow> bool) \<Rightarrow> stmt \<Rightarrow> (state \<Rightarrow> bool) \<Rightarrow> bool" ("\<Turnstile> {_} _ {_}") where
 "\<Turnstile> {P} stmt {Q} \<equiv> \<forall>S. P S \<longrightarrow> \<not>steps S stmt None \<and> (\<forall>S'. steps S stmt (Some S') \<longrightarrow> Q S')"
 
+lemma use_correct:
+  assumes "\<Turnstile> {P} stmt {Q}"
+    and "P S"
+    and "steps S stmt Sf"
+  shows "\<exists>S'. Sf = Some S' \<and> Q S'"
+  using assms by (auto simp add: correct_def)
+    (metis (full_types) not_None_eq)
+
+
 
 subsection "Weakest precondition rules"
 
@@ -24,9 +33,158 @@ lemma rule_seq:
   shows "\<Turnstile> {P} Seq a b {R}"
   using assms by (auto simp add: correct_def steps_big_seq_iff)
 
+lemma rule_if:
+  assumes "\<Turnstile> {P1} t {Q}"
+    and "\<Turnstile> {P2} f {Q}"
+  shows "\<Turnstile> {\<lambda>S. case eval S c of Some (BoolVal b) \<Rightarrow> (if b then P1 else P2) S | _ \<Rightarrow> False } If c t f {Q}"
+  using assms by (auto simp add: correct_def steps_big_if_iff split: option.splits val.splits elim: steps.cases)
 
 
 
+
+lemma steps_while_induct:
+  assumes "steps S (While c I b) Sf"
+    and "P S"
+    and loop: "\<And>S Sf. \<lbrakk>P S; eval S c = Some (BoolVal True); steps S b Sf\<rbrakk> \<Longrightarrow> \<exists>S'. Sf = Some S' \<and>  P S'"
+    and cond_wf: "\<And>S. P S \<Longrightarrow> \<exists>b. eval S c = Some (BoolVal b)"
+  shows "\<exists>S'. Sf = Some S' \<and> eval S' c = Some (BoolVal False) \<and> P S'"
+proof -
+  define stmt where "stmt \<equiv> While c I b"
+
+  have "steps S stmt Sf"
+    by (simp add: assms(1) stmt_def)
+
+  have stmt: "stmt = While c I b \<and> P S \<or> (\<exists>b'. stmt = Seq b' (While c I b) \<and> (\<forall>Sf. steps S b' Sf \<longrightarrow> (\<exists>S'. Sf = Some S' \<and>  P S')))" 
+    using stmt_def `P S` by simp
+
+  from `steps S stmt Sf` and stmt
+  have "\<exists>S'. Sf = Some S' \<and> eval S' c = Some (BoolVal False) \<and> P S'"
+  proof (induct rule: steps.induct)
+    case (final S S')
+    then show ?case
+      by (auto split: option.splits val.splits bool.splits step_res.splits)
+
+
+  next
+    case (nonfinal S stmt S' stmt' S'')
+
+    have IH1: "stmt' = While c I b \<Longrightarrow> P S'  \<Longrightarrow>
+      \<exists>S'. S'' = Some S' \<and> eval S' c = Some (BoolVal False) \<and> P S'"
+      using nonfinal.hyps by blast
+
+
+    have IH2: "\<exists>b'. stmt' = Seq b' (While c I b) \<and> (\<forall>Sf. steps S' b' Sf \<longrightarrow> (\<exists>S'. Sf = Some S' \<and> P S')) \<Longrightarrow>
+      \<exists>S'. S'' = Some S' \<and> eval S' c = Some (BoolVal False) \<and> P S'"
+      using nonfinal.hyps by blast
+
+    have IH2': "\<And>b'. stmt' = Seq b' (While c I b) \<Longrightarrow> (\<And>Sf. steps S' b' Sf \<Longrightarrow> (\<exists>S'. Sf = Some S' \<and> P S')) \<Longrightarrow>
+      \<exists>S'. S'' = Some S' \<and> eval S' c = Some (BoolVal False) \<and> P S'"
+      using nonfinal.hyps by blast
+
+    from `stmt = While c I b \<and> P S \<or>  (\<exists>b'. stmt = Seq b' (While c I b) \<and> (\<forall>Sf. steps S b' Sf \<longrightarrow> (\<exists>S'. Sf = Some S' \<and> P S')))`
+    show ?case
+    proof (rule disjE; use nothing in \<open>elim conjE exE\<close>)
+      assume "stmt = While c I b" and "P S"
+      show "\<exists>S'. S'' = Some S' \<and> eval S' c = Some (BoolVal False) \<and> P S'"
+      proof (rule IH2)
+
+
+        from `step S stmt = NonFinal S' stmt'` and `stmt = While c I b`
+        show "\<exists>b'. stmt' = Seq b' (While c I b) \<and> (\<forall>Sf. steps S' b' Sf \<longrightarrow> (\<exists>S'. Sf = Some S' \<and> P S'))"
+          apply (auto split: option.splits val.splits bool.splits)
+          using \<open>P S\<close> loop by blast+
+      qed
+    next
+      fix b'
+      assume stmt_def: "stmt = Seq b' (While c I b)"
+        and P_S': "\<forall>Sf. steps S b' Sf \<longrightarrow> (\<exists>S'. Sf = Some S' \<and> P S')"
+
+
+      from `step S stmt = NonFinal S' stmt'`
+      have "step S b' = Final S' \<and> stmt' = While c I b
+          \<or> (\<exists>b''. step S b' = NonFinal S' b'' \<and> stmt' = Seq b'' (While c I b))"
+        by (auto simp add: stmt_def split: step_res.splits)
+
+      thus "\<exists>S'. S'' = Some S' \<and> eval S' c = Some (BoolVal False) \<and> P S'"
+      proof (rule disjE; use nothing in \<open>elim conjE exE\<close>)
+        assume a0: "step S b' = Final S'"
+          and a1: "stmt' = While c I b"
+
+        show "\<exists>S'. S'' = Some S' \<and> eval S' c = Some (BoolVal False) \<and> P S'"
+          using a1
+        proof (rule IH1)
+          from P_S'
+          show "P S'"
+            by (metis a0 option.sel steps.simps)
+        qed
+      next
+        fix b''
+        assume a0: "step S b' = NonFinal S' b''"
+          and a1: "stmt' = Seq b'' (While c I b)"
+
+        show "\<exists>S'. S'' = Some S' \<and> eval S' c = Some (BoolVal False) \<and> P S'"
+          using a1
+        proof (rule IH2')
+          show "\<And>Sf. steps S' b'' Sf \<Longrightarrow> \<exists>S'. Sf = Some S' \<and> P S'"
+            by (simp add: P_S' a0 steps.nonfinal)
+        qed
+      qed
+    qed
+  next
+    case (error S)
+    then show ?case 
+      apply (auto split: option.splits val.splits bool.splits step_res.splits)
+      using cond_wf apply fastforce
+      using cond_wf apply fastforce
+      using loop steps.error by fastforce
+  qed
+
+  thus ?thesis
+    by simp
+qed
+
+lemma rule_while:
+  assumes check_body: "\<Turnstile> {P} b {\<lambda>S. eval S I = Some (BoolVal True)}"
+    and condition_wf: "\<And>S. eval S I = Some (BoolVal True) \<Longrightarrow> \<exists>b. eval S c = Some (BoolVal b)"
+    and inv_P: "\<And>S. eval S I = Some (BoolVal True) \<Longrightarrow> eval S c = Some (BoolVal True) \<Longrightarrow> P S"
+    and inv_Q: "\<And>S. eval S I = Some (BoolVal True) \<Longrightarrow> eval S c = Some (BoolVal False) \<Longrightarrow> Q S"
+  shows "\<Turnstile> {\<lambda>S. eval S I = Some (BoolVal True)} While c I b {Q}"
+proof -
+
+  have h: "\<exists>S'. Sf = Some S' \<and> eval S' c = Some (BoolVal False) \<and> eval S' I = Some (BoolVal True)"
+    if steps: "steps S (While c I b) Sf"
+      and inv_init: "eval S I = Some (BoolVal True)"
+    for S Sf
+  proof (rule steps_while_induct[OF steps])
+    show "eval S I = Some (BoolVal True)"
+      using inv_init by simp
+
+    show "\<exists>S'. Sf = Some S' \<and> eval S' I = Some (BoolVal True)"
+      if c0: "eval S I = Some (BoolVal True)"
+        and c1: "eval S c = Some (BoolVal True)"
+        and c2: "steps S b Sf"
+      for  S Sf
+    proof -
+
+      have "P S"
+        by (simp add: c0 c1 inv_P)
+
+
+      from use_correct[OF check_body `P S` `steps S b Sf`]
+      show "\<exists>S'. Sf = Some S' \<and> eval S' I = Some (BoolVal True)"
+        by blast
+    qed
+
+
+    show "\<exists>b. eval S c = Some (BoolVal b)"
+      if c0: "eval S I = Some (BoolVal True)"
+      for  S
+      by (simp add: condition_wf that)
+  qed
+
+  show ?thesis
+    using h inv_Q  by (auto simp add: correct_def)
+qed
 
 
 end
